some composition lemmas

concur/Composition.v
@@ -35,8 +35,128 @@ Unset Program Cases.
     Alloc : wt_c @ ext @ CL
  *)
 
-(**  step1 : injp @ wt_c @ injp @ wt_c @ ext @ ext @ ext @ injp @ id ==========> injp *)
+(**  step1 : injp @ wt_c @ injp @ wt_c @ ext @ ext @ ext @ injp @ id ==========> wt_c @ injp *)
 
+(**  1. injp @ wt_c @ injp @ wt_c @ ext @ injp 
+     2. wt_c @ injp @ injp @ wt_c @ ext @ injp              
+     3. wt_c @ injp @ wt_c @ ext @ injp
+     4. wt_c @ wt_c @ injp @ ext @ injp
+     5. wt_c @ injp @ ext @ injp 
+*)
 (** lemmas about [wt_c] *)
+
+Search invariant callconv.
+
+Program Coercion cc_inv {li : language_interface} (I : invariant li) : GS.callconv li li :=
+  {|
+    GS.ccworld := inv_world I;
+    GS.ccworld_world := world_unit;
+    GS.match_senv := fun w => rel_inv (symtbl_inv I w);
+    GS.match_query := fun w => rel_inv (query_inv I w);
+    GS.match_reply := fun w => rel_inv (reply_inv I w)
+  |}.
+Next Obligation.
+  inv H. reflexivity.
+Qed.
+Next Obligation.
+  inv H. auto.
+Qed.
+
+
+Infix "@" := GS.cc_compose (at level 30, right associativity).
+
+Search cctrans.
+
+Inductive match_wt_1 : (injp_world * (unit * injp_world)) -> (unit * (injp_world * injp_world)) -> Prop :=
+|match_wt_1_intro w1 w2 tt:
+  match_wt_1 (w1, (tt, w2)) (tt, (w1, w2)).
+
+Lemma move_wt_injp : cctrans (c_injp @ wt_c @ c_injp) (wt_c @ c_injp @ c_injp).
+Proof.
+  econstructor. instantiate (1:= match_wt_1).
+  - red. intros. rename se2 into se3. rename q2 into q3.
+    simpl in w2. destruct w2 as [se1'1 [ [se1'2 sig] [se2 [w1 w2]]]].
+    destruct H as [Hsei [Hse1 Hse2]]. inv Hsei. inv H. rename se1'1 into se1.
+    destruct H0 as [q1' [Hqi [q2 [Hq1 Hq2]]]]. inv Hqi. rename q1' into q1.
+    exists (se2, (w1,(se2,((se2,sig) ,w2)))). intuition auto.
+    + constructor. auto. constructor. constructor. constructor. auto.
+    + exists q2. constructor. auto. exists q2. constructor. simpl. econstructor.
+      admit. (*should be correct, can be found from old proofs*)
+      auto.
+    + constructor.
+    + destruct wp1' as [w1' [ss w2']]. destruct ss.
+      destruct H1 as [ACCE1 [_ ACCE2]]. simpl in ACCE1, ACCE2.
+      inv H0. rename w0 into wp1. rename w3 into wp2.
+      destruct H2 as [ACCI1 [_ ACCI2]]. simpl in ACCI1, ACCI2.
+      exists (tt, (w1', w2')). intuition auto.
+      repeat constructor; eauto.
+      repeat constructor; eauto. rename r2 into r3.
+      destruct H3 as [r2' [Hr1 [r2 [Hri Hr2]]]]. inv Hri.
+      repeat econstructor; eauto.
+      simpl. simpl in H0.
+      admit.
+  - red. intros.  rename se2 into se3. rename q2 into q3.
+    simpl in wp1. rename wp2 into xxx.
+    destruct wp1 as [wp1 [ss wp2]]. destruct ss. inv H2. simpl in w1.
+    destruct w1 as [se2' [w1 [se2 [[se2'' sig] w2]]]].
+    destruct H1 as [ACCI1 [X ACCI2]]. simpl in ACCI1, ACCI2. inv X.
+    destruct H as [Hse1 [Hsei Hse2]]. inv Hsei. inv H.
+    destruct H0 as [q2 [Hq1 [q2' [Hqi Hq2]]]]. inv Hqi. rename q2' into q2.
+    exists (se1,((se1,sig),(se2,(w1,w2)) )). intuition auto.
+    + repeat constructor; auto.
+    + repeat constructor; auto.
+    + exists q1. constructor. admit.
+      exists q2. constructor; auto.
+    + destruct wp2' as [ss [wp1' wp2']]. destruct ss.
+      destruct H0 as [x [E1 E2]]. simpl in x,E1,E2. rename r2 into r3.
+      destruct H1 as [r1' [Hri [r2 [Hr1 Hr2]]]]. inv Hri.
+      exists (wp1', (tt, wp2')). intuition auto.
+      repeat constructor; auto.
+      exists r2. split; auto. exists r2. split; auto. admit.
+      constructor.
+Admitted.
+
+Inductive match_assoc_1 {A B C : Type}: (A * (B * C)) -> (A * B * C) -> Prop :=
+|match_assoc_1_intro a b c: match_assoc_1 (a,(b,c)) (a,b,c).
+
+Lemma cc_compose_assoc {A B C D}:
+  forall (cc1 : GS.callconv A B) (cc2 : GS.callconv B C) (cc3 : GS.callconv C D),
+    cctrans (cc1 @ cc2 @ cc3) ((cc1 @ cc2) @ cc3).
+Proof.
+  econstructor. instantiate (1:= match_assoc_1).
+  - red.
+    intros [sec [[seb [w1 w2]] w3]] sea sed qa qd.
+    intros ((Hseab & Hsebc) & Hsecd) (qc & (qb & Hqab & Hqbc) & Hqcd).
+    exists (seb, (w1, (sec, (w2, w3)))). intuition auto.
+    repeat constructor; auto.
+    repeat econstructor; eauto. simpl.
+    constructor. 
+    destruct wp1' as [w1' [w2' w3']].
+    rename wp2 into wp2'.
+    destruct wp1 as [wp1 [wp2 wp3]]. inv H.
+    destruct H0 as [E1 [E2 E3]]. destruct H1 as [I1 [I2 I3]]. simpl in E1,E2,E3,I1,I2,I3.
+    exists ((w1',w2'),w3'). intuition auto.
+    repeat constructor; auto.
+    repeat constructor; auto.
+    destruct H2 as [rb [Hr1 [rc [Hr2 Hr3]]]].
+    repeat econstructor; eauto.
+  - red.
+    intros [w1 [w2 w3]] [[wp1 wp2] wp3] [seb [w1' [sec [w2' w3']]]]
+    sea sed qa qd.
+    intros (Hseab & Hsebc & Hsecd) (qb & Hqab & qc & Hqbc & Hqcd) [I1 [I2 I3]] Hm.
+    simpl in I1, I2, I3. inv Hm.
+    exists (sec,(seb,(w1', w2'),w3')). intuition auto.
+    repeat constructor; auto.
+    repeat econstructor; eauto.
+    repeat econstructor; eauto.
+    simpl in H. destruct wp2' as [[w1'' w2''] w3''].
+    destruct H as [[E1 E2]E3]. simpl in E1, E2, E3.
+    exists (w1'', (w2'', w3'')). intuition auto.
+    repeat constructor; auto.
+    destruct H0 as [rc [[rb [Hr1 Hr2]] Hr3]].
+    repeat econstructor; eauto.
+    constructor.
+Qed.
+
 
 
